wip, refactoring

pulse/examples/dsls/mini_steel/Pulse.Elaborate.Core.fst
@@ -222,181 +222,176 @@ let mk_sub_stt_ghost (u:R.universe) (a opened pre1 pre2 post1 post2 e:R.term)  =
   let t = pack_ln (R.Tv_App t (`(), Q_Explicit)) in
   pack_ln (R.Tv_App t (e, Q_Explicit))
 
-let elab_frame (c:pure_comp_st) (frame:pure_term) (e:R.term) =
+let elab_frame (c:comp_st) (frame:term) (e:R.term) =
   let u = elab_universe (comp_u c) in
-  let ty = elab_pure (comp_res c) in
-  let pre = elab_pure (comp_pre c) in
-  let post = elab_pure (comp_post c) in
+  let ty = elab_term (comp_res c) in
+  let pre = elab_term (comp_pre c) in
+  let post = elab_term (comp_post c) in
   if C_ST? c
-  then mk_frame_stt u ty pre (mk_abs ty R.Q_Explicit post) (elab_pure frame) e
-  else let opened = elab_pure (comp_inames c) in      
+  then mk_frame_stt u ty pre (mk_abs ty R.Q_Explicit post) (elab_term frame) e
+  else let opened = elab_term (comp_inames c) in      
        if C_STAtomic? c
-       then mk_frame_stt_atomic u ty opened pre (mk_abs ty R.Q_Explicit post) (elab_pure frame) e
+       then mk_frame_stt_atomic u ty opened pre (mk_abs ty R.Q_Explicit post) (elab_term frame) e
        else let _ = assert (C_STGhost? c) in
-            mk_frame_stt_ghost u ty opened pre (mk_abs ty R.Q_Explicit post) (elab_pure frame) e
+            mk_frame_stt_ghost u ty opened pre (mk_abs ty R.Q_Explicit post) (elab_term frame) e
 
-let elab_sub (c1 c2:pure_comp_st) (e:R.term) =
-  let ty = elab_pure (comp_res c1) in
+let elab_sub (c1 c2:comp_st) (e:R.term) =
+  let ty = elab_term (comp_res c1) in
   let u = elab_universe (comp_u c1) in
-  let pre1 = elab_pure (comp_pre c1) in
-  let pre2 = elab_pure (comp_pre c2) in
-  let post1 = mk_abs ty R.Q_Explicit (elab_pure (comp_post c1)) in
-  let post2 = mk_abs ty R.Q_Explicit (elab_pure (comp_post c2)) in
+  let pre1 = elab_term (comp_pre c1) in
+  let pre2 = elab_term (comp_pre c2) in
+  let post1 = mk_abs ty R.Q_Explicit (elab_term (comp_post c1)) in
+  let post2 = mk_abs ty R.Q_Explicit (elab_term (comp_post c2)) in
   if C_ST? c1
   then mk_sub_stt u ty pre1 pre2 post1 post2 e
-  else let opened = elab_pure (comp_inames c1) in
+  else let opened = elab_term (comp_inames c1) in
        if C_STAtomic? c1
        then mk_sub_stt_atomic u ty opened pre1 pre2 post1 post2 e
        else let _ = assert (C_STGhost? c1) in
             mk_sub_stt_ghost u ty opened pre1 pre2 post1 post2 e
 
-#push-options "--z3rlimit_factor 4"
-let rec elab_bind #f #g #x #c1 #c2 #c
-  (bc:bind_comp f g x c1 c2 c)
-  (e1 e2:R.term)
-  : Tot R.term (decreases bc) =
 
-  let t1 = elab_pure (comp_res c1) in
-  let t2 = elab_pure (comp_res c2) in
-
-  match bc with
-  | Bind_comp _ _ _ _ _ _ _ ->
-    if C_ST? c1
-    then
-      mk_bind_stt
+let elab_bind #f #g #x #c1 #c2 #c
+              (bc:bind_comp f g x c1 c2 c)
+              (e1 e2:R.term)
+  : R.term
+  = let t1 = elab_term (comp_res c1) in
+    let t2 = elab_term (comp_res c2) in
+    match bc with
+    | Bind_comp _ _ _ _ _ _ _ ->
+      if C_ST? c1
+      then
+        mk_bind_stt
+          (elab_universe (comp_u c1))
+          (elab_universe (comp_u c2))
+          t1 t2
+          (elab_term (comp_pre c1))
+          (mk_abs t1 R.Q_Explicit (elab_term (comp_post c1)))
+          (mk_abs t2 R.Q_Explicit (elab_term (comp_post c2)))
+          e1 e2
+      else 
+        mk_bind_ghost
+          (elab_universe (comp_u c1))
+          (elab_universe (comp_u c2))
+          t1 t2
+          (elab_term (comp_inames c1))
+          (elab_term (comp_pre c1))
+          (mk_abs t1 R.Q_Explicit (elab_term (comp_post c1)))
+          (mk_abs t2 R.Q_Explicit (elab_term (comp_post c2)))
+          e1 e2
+  
+    | Bind_comp_ghost_l _ _ _ _ (| reveal_a, reveal_a_typing |) _ _ _ ->
+      mk_bind_ghost_atomic
         (elab_universe (comp_u c1))
         (elab_universe (comp_u c2))
         t1 t2
-        (elab_pure (comp_pre c1))
-        (mk_abs t1 R.Q_Explicit (elab_pure (comp_post c1)))
-        (mk_abs t2 R.Q_Explicit (elab_pure (comp_post c2)))
+        (elab_term (comp_inames c1))
+        (elab_term (comp_pre c1))
+        (mk_abs t1 R.Q_Explicit (elab_term (comp_post c1)))
+        (mk_abs t2 R.Q_Explicit (elab_term (comp_post c2)))
         e1 e2
-    else 
-      mk_bind_ghost
+        (elab_term reveal_a)
+
+    | Bind_comp_ghost_r _ _ _ _ (| reveal_b, reveal_b_typing |) _ _ _ ->
+      mk_bind_atomic_ghost
         (elab_universe (comp_u c1))
         (elab_universe (comp_u c2))
         t1 t2
-        (elab_pure (comp_inames c1))
-        (elab_pure (comp_pre c1))
-        (mk_abs t1 R.Q_Explicit (elab_pure (comp_post c1)))
-        (mk_abs t2 R.Q_Explicit (elab_pure (comp_post c2)))
+        (elab_term (comp_inames c1))
+        (elab_term (comp_pre c1))
+        (mk_abs t1 R.Q_Explicit (elab_term (comp_post c1)))
+        (mk_abs t2 R.Q_Explicit (elab_term (comp_post c2)))
         e1 e2
+        (elab_term reveal_b)
 
-  | Bind_comp_ghost_l _ _ _ _ (| reveal_a, reveal_a_typing |) _ _ _ ->
-    mk_bind_ghost_atomic
-      (elab_universe (comp_u c1))
-      (elab_universe (comp_u c2))
-      t1 t2
-      (elab_pure (comp_inames c1))
-      (elab_pure (comp_pre c1))
-      (mk_abs t1 R.Q_Explicit (elab_pure (comp_post c1)))
-      (mk_abs t2 R.Q_Explicit (elab_pure (comp_post c2)))
-      e1 e2
-      (elab_src_typing reveal_a_typing)
-
-  | Bind_comp_ghost_r _ _ _ _ (| reveal_b, reveal_b_typing |) _ _ _ ->
-    mk_bind_atomic_ghost
-      (elab_universe (comp_u c1))
-      (elab_universe (comp_u c2))
-      t1 t2
-      (elab_pure (comp_inames c1))
-      (elab_pure (comp_pre c1))
-      (mk_abs t1 R.Q_Explicit (elab_pure (comp_post c1)))
-      (mk_abs t2 R.Q_Explicit (elab_pure (comp_post c2)))
-      e1 e2
-      (elab_src_typing reveal_b_typing)
-
-and elab_lift #f #g #c1 #c2 (d:lift_comp f g c1 c2) (e:R.term)
-  : Tot R.term (decreases d) =
-
-  match d with
-  | Lift_STAtomic_ST _ _ ->
-    let t = elab_pure (comp_res c1) in
-    mk_lift_atomic_stt
-      (elab_universe (comp_u c1))
-      (elab_pure (comp_res c1))
-      t
-      (mk_abs t R.Q_Explicit (elab_pure (comp_post c1)))
-      e
-      
-  | Lift_STGhost_STAtomic _ _ (| reveal_a, reveal_a_typing |) ->
-    let t = elab_pure (comp_res c1) in
-    mk_lift_ghost_atomic
-      (elab_universe (comp_u c1))
-      t
-      (elab_pure (comp_inames c1))
-      (elab_pure (comp_pre c1))
-      (mk_abs t R.Q_Explicit (elab_pure (comp_post c1)))
-      e
-      (elab_src_typing reveal_a_typing)
-
-and elab_src_typing
-  (#f:RT.fstar_top_env)
-  (#g:env)
-  (#t:term)
-  (#c:pure_comp)
-  (d:src_typing f g t c)
-  : Tot R.term (decreases d)
-
+let elab_lift #f #g #c1 #c2 (d:lift_comp f g c1 c2) (e:R.term)
+  : Tot R.term
   = match d with
-    | T_Tot _ _ _ _ -> elab_pure t
+    | Lift_STAtomic_ST _ _ ->
+      let t = elab_term (comp_res c1) in
+      mk_lift_atomic_stt
+        (elab_universe (comp_u c1))
+        (elab_term (comp_res c1))
+        t
+        (mk_abs t R.Q_Explicit (elab_term (comp_post c1)))
+        e
+        
+    | Lift_STGhost_STAtomic _ _ (| reveal_a, reveal_a_typing |) ->
+      let t = elab_term (comp_res c1) in
+      mk_lift_ghost_atomic
+        (elab_universe (comp_u c1))
+        t
+        (elab_term (comp_inames c1))
+        (elab_term (comp_pre c1))
+        (mk_abs t R.Q_Explicit (elab_term (comp_post c1)))
+        e
+        (elab_term reveal_a)
 
-    | T_Abs _ ppname x qual ty _u body _c ty_typing body_typing ->
-      let ty = elab_pure ty in
-      let body = elab_src_typing body_typing in
+let rec elab_st_typing (#f:RT.fstar_top_env)
+                       (#g:env)
+                       (#t:st_term)
+                       (#c:comp)
+                       (d:st_typing f g t c)
+  : Tot R.term (decreases d)
+  = match d with
+    | T_Tot _ t _ _ -> elab_term t
+
+    | T_Abs _ x qual ty _u body _c ty_typing body_typing ->
+      let ty = elab_term ty in
+      let body = elab_st_typing body_typing in
+      let ppname = (Tm_Abs?.b t).binder_ppname in
       mk_abs_with_name ppname ty (elab_qual qual) (RT.close_term body x) //this closure should be provably redundant by strengthening the conditions on x
-    
-    | T_STApp _ head _ppname _formal qual _res arg head_typing arg_typing ->
-      let head = elab_src_typing head_typing in
-      let arg = elab_pure arg in
+
+    | T_STApp _ head  _formal qual _res arg head_typing arg_typing ->
+      let head = elab_st_typing head_typing in
+      let arg = elab_term arg in
       R.mk_app head [(arg, elab_qual qual)]
 
-    | T_Return _ _ ty u _ _ ->
-      mk_return (elab_universe u) (elab_pure ty) (elab_pure t)
+    | T_Return _ e ty u _ _ ->
+      mk_return (elab_universe u) (elab_term ty) (elab_term e)
 
     | T_ReturnNoEq _ _ ty u t_typing _ ->
-      mk_return_noeq (elab_universe u) (elab_pure ty) (elab_src_typing t_typing)
+      mk_return_noeq (elab_universe u) (elab_term ty) (elab_st_typing t_typing)
 
     | T_Bind _ e1 e2 c1 c2 x c e1_typing t_typing e2_typing bc ->
-      let e1 = elab_src_typing e1_typing in
-      let e2 = elab_src_typing e2_typing in
-      let ty1 = elab_pure (comp_res c1) in
+      let e1 = elab_st_typing e1_typing in
+      let e2 = elab_st_typing e2_typing in
+      let ty1 = elab_term (comp_res c1) in
       elab_bind bc e1 (mk_abs ty1 R.Q_Explicit (RT.close_term e2 x))
       
     | T_Frame _ _ c frame _frame_typing e_typing ->
-      let e = elab_src_typing e_typing in
+      let e = elab_st_typing e_typing in
       elab_frame c frame e
       
     | T_Equiv _ _ c1 c2 e_typing _ ->
-      let e = elab_src_typing e_typing in
+      let e = elab_st_typing e_typing in
       elab_sub c1 c2 e
 
     | T_Lift _ _ c1 c2 e_typing lc ->
-      let e = elab_src_typing e_typing in
+      let e = elab_st_typing e_typing in
       elab_lift lc e
 
     | T_If _ b _ _ _ _ _ _ e1_typing e2_typing _c_typing ->
-      let rb = elab_pure b in
-      let re1 = elab_src_typing e1_typing in
-      let re2 = elab_src_typing e2_typing in
+      let rb = elab_term b in
+      let re1 = elab_st_typing e1_typing in
+      let re2 = elab_st_typing e2_typing in
       RT.mk_if rb re1 re2
 
     | T_ElimExists _ u t p _ d_t d_exists ->
       let ru = elab_universe u in
-      let rt = elab_pure t in
-      let rp = elab_pure p in
+      let rt = elab_term t in
+      let rp = elab_term p in
       mk_elim_exists ru rt (mk_abs rt R.Q_Explicit rp)
 
     | T_IntroExists _ u t p e _ _ _ ->
       let ru = elab_universe u in
-      let rt = elab_pure t in
-      let rp = elab_pure p in
-      let re = elab_pure e in
+      let rt = elab_term t in
+      let rp = elab_term p in
+      let re = elab_term e in
       mk_intro_exists ru rt (mk_abs rt R.Q_Explicit rp) re
 
     | T_While _ inv _ _ _ cond_typing body_typing ->
-      let inv = elab_pure inv in
-      let cond = elab_src_typing cond_typing in
-      let body = elab_src_typing body_typing in
+      let inv = elab_term inv in
+      let cond = elab_st_typing cond_typing in
+      let body = elab_st_typing body_typing in
       mk_while (mk_abs bool_tm R.Q_Explicit inv) cond body
-#pop-options
