pulse/examples/dsls/mini_steel/Pulse.Typing.LN.fsti
@@ -6,6 +6,10 @@ open FStar.List.Tot
 open Pulse.Syntax
 open Pulse.Typing
 
-val src_typing_ln (#f:_) (#g:_) (#t:_) (#c:_)
-                  (d:src_typing f g t c)
-  : Lemma (ln t /\ ln_c c)
+val tot_typing_ln (#f:_) (#g:_) (#e:_) (#t:_)
+                  (d:tot_typing f g e t)
+  : Lemma (ln e /\ ln t)
+
+val st_typing_ln (#f:_) (#g:_) (#t:_) (#c:_)
+                 (d:st_typing f g t c)
+  : Lemma (ln_st t /\ ln_c c)
